Deploying to gh-pages from @ xubaiw/reservoir-index@a904eca4c99dd9852d69a14cdc6342f281013705 🚀

git/cruhland/lean4-axiomatic/Lean4Axiomatic/Integer/Impl/Difference.lean
@@ -161,10 +161,10 @@ instance addOp : Add (Difference ℕ) := {
 Addition of natural number differences is commutative.
 
 **Proof intuition**: Expand definitions to see that we need to show the
-equivalence of two differences of natural number sums. The left and right sides
-of the differences are directly equivalent via commutativity of natural number
-addition, so convert the differences into ordered pairs and use commutativity
-element-wise.
+equivalence of two differences of natural number sums. The left and right
+elements of the differences are directly equivalent via commutativity of
+natural number addition, so convert the differences into ordered pairs and use
+commutativity element-wise.
 -/
 theorem add_comm {a b : Difference ℕ} : a + b ≃ b + a := by
   revert a; intro (a₁——a₂); revert b; intro (b₁——b₂)
@@ -255,8 +255,83 @@ instance mulOp : Mul (Difference ℕ) := {
   mul := mul
 }
 
+/--
+Multiplication of natural number differences is commutative.
+
+**Proof intuition**: Expand definitions to see that we need to show the
+equivalence of two differences of natural number sums of products. The left and
+right elements of the differences are directly equivalent via commutativity of
+natural number addition and multiplication, so convert the differences into
+ordered pairs and use commutativity element-wise.
+-/
+theorem mul_comm {a b : Difference ℕ} : a * b ≃ b * a := by
+  revert a; intro (n——m); revert b; intro (k——j)
+  show n——m * k——j ≃ k——j * n——m
+  show (n * k + m * j)——(n * j + m * k) ≃ (k * n + j * m)——(k * m + j * n)
+  show from_prod (n * k + m * j, n * j + m * k)
+     ≃ from_prod (k * n + j * m, k * m + j * n)
+  apply AA.subst₁
+  show (n * k + m * j, n * j + m * k) ≃ (k * n + j * m, k * m + j * n)
+  calc
+    (n * k + m * j, n * j + m * k) ≃ _ := AA.substL (AA.substL AA.comm)
+    (k * n + m * j, n * j + m * k) ≃ _ := AA.substL (AA.substR AA.comm)
+    (k * n + j * m, n * j + m * k) ≃ _ := AA.substR (AA.substL AA.comm)
+    (k * n + j * m, j * n + m * k) ≃ _ := AA.substR (AA.substR AA.comm)
+    (k * n + j * m, j * n + k * m) ≃ _ := AA.substR AA.comm
+    (k * n + j * m, k * m + j * n) ≃ _ := Rel.refl
+
+instance mul_commutative : AA.Commutative (α := Difference ℕ) (· * ·) := {
+  comm := mul_comm
+}
+
+/--
+Multiplying the same difference on the right of two equivalent differences
+preserves their equivalence.
+
+**Proof intuition**: The property is already intuitively true; imagine
+stretching two line segments of the same length by the same amount. So the
+proof just expands all definitions into equalities of sums of products of
+natural numbers, and performs algebra to obtain the desired result.
+-/
+theorem mul_substL {a₁ a₂ b : Difference ℕ} : a₁ ≃ a₂ → a₁ * b ≃ a₂ * b := by
+  revert a₁; intro (n——m); revert a₂; intro (k——j); revert b; intro (p——q)
+  intro (_ : n——m ≃ k——j)
+  have h : n + j ≃ k + m := ‹n——m ≃ k——j›
+  show n——m * p——q ≃ k——j * p——q
+  show (n * p + m * q)——(n * q + m * p) ≃ (k * p + j * q)——(k * q + j * p)
+  show (n * p + m * q) + (k * q + j * p) ≃ (k * p + j * q) + (n * q + m * p)
+  calc
+    (n * p + m * q) + (k * q + j * p) ≃ _ := Rel.symm expand_swap
+    (n + j) * p     + (k + m) * q     ≃ _ := AA.substL (AA.substL h)
+    (k + m) * p     + (k + m) * q     ≃ _ := AA.substR (AA.substL (Rel.symm h))
+    (k + m) * p     + (n + j) * q     ≃ _ := expand_swap
+    (k * p + j * q) + (n * q + m * p) ≃ _ := Rel.refl
+where
+  expand_swap
+      {u v w x y z : ℕ}
+      : (w + x) * u + (y + z) * v ≃ (w * u + z * v) + (y * v + x * u)
+      := calc
+    (w + x) * u     + (y + z) * v     ≃ _ := AA.substL AA.distribR
+    (w * u + x * u) + (y + z) * v     ≃ _ := AA.substR AA.distribR
+    (w * u + x * u) + (y * v + z * v) ≃ _ := AA.expr_xxfxxff_lr_swap_rr
+    (w * u + z * v) + (y * v + x * u) ≃ _ := Rel.refl
+
+def mul_substitutiveL
+    : AA.SubstitutiveOn
+      Hand.L (α := Difference ℕ) (· * ·) AA.tc (· ≃ ·) (· ≃ ·) := {
+  subst₂ := λ (_ : True) => mul_substL
+}
+
+def mul_substitutive
+    : AA.Substitutive₂ (α := Difference ℕ) (· * ·) AA.tc (· ≃ ·) (· ≃ ·) := {
+  substitutiveL := mul_substitutiveL
+  substitutiveR := AA.substR_from_substL_swap (rS := (· ≃ ·)) mul_substitutiveL
+}
+
 def multiplication : Multiplication.Base (Difference ℕ) := {
   mulOp := mulOp
+  mul_commutative := mul_commutative
+  mul_substitutive := mul_substitutive
 }
 
 instance integer : Integer (Difference ℕ) := {
