git/cruhland/lean4-analysis/Lean4Analysis/Ch4/Ch4Sec1Integers.lean
@@ -10,7 +10,9 @@ abbrev ℕ : Type := Nat
 
 namespace Impl
 
-export Integer.Impl.Difference (addition equality multiplication)
+export Integer.Impl.Difference (
+  addition equality from_prod from_prod_substitutive multiplication
+)
 
 end Impl
 
@@ -33,7 +35,7 @@ example {a b c d : ℕ} : a——b ≃ c——d ↔ a + d ≃ c + b := Iff.intro
 -- `3 + 4 ≃ 2 + 5`.
 example : 3——5 ≃ 2——4 := by
   show 3 + 4 ≃ 2 + 5
-  exact Eqv.refl
+  exact Rel.refl
 
 -- On the other hand, `3——5` is not equal to `2——3` because `3 + 3 ≄ 2 + 5`.
 example : 3——5 ≄ 2——3 := by
@@ -67,5 +69,70 @@ example {a b c d : ℕ} : a——b * c——d ≃ (a * c + b * d)——(a * d + 
 
 -- [definition of integer multiplication]
 example : ℤ → ℤ → ℤ := Impl.multiplication.mulOp.mul
+
+-- Thus for instance, `(3——5) + (1——4)` is equal to `(4——9)`.
+example : (3——5) + (1——4) ≃ (4——9) := rfl
+
+-- There is however one thing we have to check before we can accept these
+-- definitions - we have to check that if we replace one of the integers by an
+-- equal integer, that the sum or product does not change. For instance,
+-- `(3——5)` is equal to `(2——4)`, so `(3——5) + (1——4)` ought to have the same
+-- value as `(2——4) + (1——4)`, otherwise this would not give a consistent
+-- definition of addition.
+example : (3——5) ≃ (2——4) := rfl
+
+example : (3——5) + (1——4) ≃ (2——4) + (1——4) := rfl
+
+-- Lemma 4.1.3 (Addition and multiplication are well-defined).
+-- Let `a`, `b`, `a'`, `b'`, `c`, `d` be natural numbers. If
+-- `(a——b) ≃ (a'——b')`, then `(a——b) + (c——d) ≃ (a'——b') + (c——d)` and
+-- `(a——b) * (c——d) ≃ (a'——b') * (c——d)`, and also
+-- `(c——d) + (a——b) ≃ (c——d) + (a'——b')` and
+-- `(c——d) * (a——b) ≃ (c——d) * (a'——b')`. Thus addition and multiplication are
+-- well-defined operations (equal inputs give equal outputs).
+section lemma_4_1_3
+
+variable {a b a' b' c d : ℕ}
+variable (_ : (a——b) ≃ (a'——b'))
+
+example : (a——b) + (c——d) ≃ (a'——b') + (c——d) :=
+  AA.substL
+    (self := Impl.addition.add_substitutive.substitutiveL)
+    ‹(a——b) ≃ (a'——b')›
+
+example : (a——b) * (c——d) ≃ (a'——b') * (c——d) :=
+  AA.substL
+    (self := Impl.multiplication.mul_substitutive.substitutiveL)
+    ‹(a——b) ≃ (a'——b')›
+
+example : (c——d) + (a——b) ≃ (c——d) + (a'——b') :=
+  AA.substR
+    (self := Impl.addition.add_substitutive.substitutiveR)
+    ‹(a——b) ≃ (a'——b')›
+
+example : (c——d) * (a——b) ≃ (c——d) * (a'——b') :=
+  AA.substR
+    (self := Impl.multiplication.mul_substitutive.substitutiveR)
+    ‹(a——b) ≃ (a'——b')›
+
+end lemma_4_1_3
+
+-- The integers `n——0` behave in the same way as the natural numbers `n`;
+-- indeed one can check that `(n——0) + (m——0) ≃ (n + m)——0` and
+-- `(n——0) * (m——0) ≃ (n * m)——0`.
+example {n m : ℕ} : (n——0) + (m——0) ≃ (n + m)——0 := rfl
+
+example {n m : ℕ} : (n——0) * (m——0) ≃ (n * m)——0 := by
+  show (n * m + 0 * 0)——(n * 0 + 0 * m) ≃ (n * m)——0
+  show Impl.from_prod (n * m + 0 * 0, n * 0 + 0 * m) ≃ Impl.from_prod (n * m, 0)
+  apply AA.subst₁ (self := Impl.from_prod_substitutive)
+  show (n * m + 0 * 0, n * 0 + 0 * m) ≃ (n * m, 0)
+  calc
+    (n * m + 0 * 0, n * 0 + 0 * m) ≃ _ := AA.substL (AA.substR Natural.zero_mul)
+    (n * m + 0, n * 0 + 0 * m)     ≃ _ := AA.substL Natural.add_zero
+    (n * m, n * 0 + 0 * m)         ≃ _ := AA.substR (AA.substL Natural.mul_zero)
+    (n * m, 0 + 0 * m)             ≃ _ := AA.substR Natural.zero_add
+    (n * m, 0 * m)                 ≃ _ := AA.substR Natural.zero_mul
+    (n * m, 0)                     ≃ _ := Rel.refl
 
 end AnalysisI.Ch4.Sec1
