git/cruhland/lean4-axiomatic/Lean4Axiomatic/AbstractAlgebra.lean
@@ -70,8 +70,7 @@ class DistributiveOn
   - `z`: the right argument to `g`.
   -/
   distrib {x y z : α} :
-    let f' := hand.align f
-    f' x (g y z) ≃ g (f' x y) (f' x z)
+    hand.align f x (g y z) ≃ g (hand.align f x y) (hand.align f x z)
 
 export DistributiveOn (distrib)
 
@@ -118,7 +117,7 @@ def distributiveR_from_distributiveL
     : DistributiveOn Hand.L f g → DistributiveOn Hand.R f g := by
   intro
   constructor
-  intro x y z f'
+  intro x y z
   show f (g y z) x ≃ g (f y x) (f z x)
   calc
     f (g y z) x       ≃ _ := AA.comm
@@ -160,12 +159,39 @@ The sort `α` and its binary operation `f` must form a commutative semigroup.
 theorem expr_xxfxxff_lr_swap_rl
     {α : Sort u} {f : α → α → α} {a b c d : α} [EqvOp α]
     [Associative f] [Commutative f] [Substitutive₂ f tc (· ≃ ·) (· ≃ ·)]
-    : f (f a b) (f c d) ≃ f (f a c) (f b d) := calc
+    : f (f a b) (f c d) ≃ f (f a c) (f b d)
+    := calc
   f (f a b) (f c d) ≃ _ := AA.assoc
   f a (f b (f c d)) ≃ _ := AA.substR (Rel.symm AA.assoc)
   f a (f (f b c) d) ≃ _ := AA.substR (AA.substL AA.comm)
   f a (f (f c b) d) ≃ _ := AA.substR AA.assoc
   f a (f c (f b d)) ≃ _ := Rel.symm AA.assoc
   f (f a c) (f b d) ≃ _ := Rel.refl
+
+/--
+Swaps the second and fourth elements of a balanced four-element expression
+involving a single binary operation.
+
+The sort `α` and its binary operation `f` must form a commutative semigroup.
+
+**Named parameters**
+- `α`: the sort over which `f` operates.
+- `f`: the binary operation used in the expression.
+- `a`, `b`, `c`, `d`: the operands to `f` in the expression.
+
+**Class parameters**
+- `EqvOp α`: needed to express the identity between expressions.
+- `Associative f`, `Commutative f`: needed to rearrange the operands freely.
+- `Substitutive₂ f tc (· ≃ ·) (· ≃ ·)`: needed to rearrange subexpressions.
+-/
+theorem expr_xxfxxff_lr_swap_rr
+    {α : Sort u} {f : α → α → α} {a b c d : α} [EqvOp α]
+    [Associative f] [Commutative f] [Substitutive₂ f tc (· ≃ ·) (· ≃ ·)]
+    : f (f a b) (f c d) ≃ f (f a d) (f c b)
+    := calc
+  f (f a b) (f c d) ≃ _ := AA.substR AA.comm
+  f (f a b) (f d c) ≃ _ := expr_xxfxxff_lr_swap_rl
+  f (f a d) (f b c) ≃ _ := AA.substR AA.comm
+  f (f a d) (f c b) ≃ _ := Rel.refl
 
 end Lean4Axiomatic.AA
