git/cruhland/lean4-axiomatic/Lean4Axiomatic/Integer/Multiplication.lean
@@ -1,3 +1,5 @@
+import Lean4Axiomatic.AbstractAlgebra
+import Lean4Axiomatic.Integer.Core
 
 namespace Lean4Axiomatic.Integer
 
@@ -10,9 +12,18 @@ Definition of multiplication, and properties that it must satisfy.
 
 All other properties of multiplication can be derived from these.
 -/
-class Multiplication.Base (ℤ : Type) :=
+class Multiplication.Base (ℤ : Type) [Core ℤ] :=
   /-- Definition of and syntax for multiplication. -/
   mulOp : Mul ℤ
+
+  /--
+  Multiplication preserves equality of integers; two equal integers are still
+  equal after the same quantity is multiplied with both (on the left or right).
+  -/
+  mul_substitutive : AA.Substitutive₂ (α := ℤ) (· * ·) AA.tc (· ≃ ·) (· ≃ ·)
+
+  /-- Exchanging the operands of multiplication does not change the result. -/
+  mul_commutative : AA.Commutative (α := ℤ) (· * ·)
 
 namespace Multiplication
 export Multiplication.Base (mulOp)
